TestModels/Aggregate/test/SimpleAggregateImplTest.dfy
@@ -7,6 +7,7 @@ module SimpleAggregateImplTest {
     method{:test} GetAggregate(){
         var client :- expect SimpleAggregate.SimpleAggregate();
         TestGetAggregate(client);
+        TestGetAggregateKnownValue(client);
     }
 
     method TestGetAggregate(client: ISimpleAggregateClient)
@@ -30,5 +31,30 @@ module SimpleAggregateImplTest {
         expect ret.simpleStringMap.UnwrapOr(map[]) == simpleStringMap;
         expect ret.simpleIntegerMap.UnwrapOr(map[]) == simpleIntegerMap;
         expect ret.nestedStructure.UnwrapOr(NestedStructure(stringStructure := Some(StringStructure(value := Some(""))))) == nestedStructure;
+        print ret;
+    }
+
+    method TestGetAggregateKnownValue(client: ISimpleAggregateClient)
+    requires client.ValidState()
+      modifies client.Modifies
+      ensures client.ValidState()
+      {
+        var stringList := ["Test"];
+        var simpleStringMap := map["Test1" := "Success"];
+        var structureList :=[StructureListElement(stringValue := Some("Test2"), integerValue := Some(2))];
+        var simpleIntegerMap := map["Test3" := 3];
+        var nestedStructure := NestedStructure(stringStructure := Some(StringStructure(value := Some("Nested"))));
+        var ret :- expect client.GetAggregate(GetAggregateInput(simpleIntegerMap := Some(simpleIntegerMap),
+                                                                simpleStringMap := Some(simpleStringMap),
+                                                                simpleStringList := Some(stringList),
+                                                                structureList := Some(structureList),
+                                                                nestedStructure := Some(nestedStructure))
+                                                                );
+        expect ret.simpleStringList.UnwrapOr([]) == stringList;
+        expect ret.structureList.UnwrapOr([]) == structureList;
+        expect ret.simpleStringMap.UnwrapOr(map[]) == simpleStringMap;
+        expect ret.simpleIntegerMap.UnwrapOr(map[]) == simpleIntegerMap;
+        expect ret.nestedStructure.UnwrapOr(NestedStructure(stringStructure := Some(StringStructure(value := Some(""))))) == nestedStructure;
+        print ret;
     }
 }
