TestModels/Aggregate/Model/aggregate.smithy
@@ -7,13 +7,18 @@ namespace simple.aggregate
 service SimpleAggregate {
   version: "2021-11-01",
   resources: [],
-  operations: [ GetAggregate ],
+  operations: [ GetAggregate, GetAggregateKnownValueTest ],
   errors: [],
 }
 
 structure SimpleAggregateConfig {}
 
 operation GetAggregate {
+  input: GetAggregateInput,
+  output: GetAggregateOutput,
+}
+
+operation GetAggregateKnownValueTest {
   input: GetAggregateInput,
   output: GetAggregateOutput,
 }
